lean/Runtime/Shim/GenHeap.lean
@@ -13,22 +13,24 @@ set_option autoImplicit false
 
 /-! ## Generalized Heap -/
 
-axiom HeapLookup {Λ : Type} [Language Λ] : Language.state Λ → Nat → Option (Language.val Λ)
-axiom HeapInsert {Λ : Type} [Language Λ] : Language.state Λ → Nat → Language.val Λ → Language.state Λ
+axiom HeapLookup {Λ : Type} [Iris.Language Λ] :
+    Iris.Language.state Λ → Nat → Option (Iris.Language.val Λ)
+axiom HeapInsert {Λ : Type} [Iris.Language Λ] :
+    Iris.Language.state Λ → Nat → Iris.Language.val Λ → Iris.Language.state Λ
 
-axiom pointsto {Λ : Type} [Language Λ] (l : Nat) (v : Language.val Λ) : iProp
+axiom pointsto {Λ : Type} [Iris.Language Λ] (l : Nat) (v : Iris.Language.val Λ) : iProp
 
-axiom gen_heap_alloc {Λ : Type} [Language Λ] (σ : Language.state Λ)
-    (l : Nat) (v : Language.val Λ) (hFresh : HeapLookup σ l = none) :
-    iProp.entails (state_interp Λ σ)
-      (bupd (iProp.sep (state_interp Λ (HeapInsert σ l v)) (pointsto l v)))
+axiom gen_heap_alloc {Λ : Type} [Iris.Language Λ] (σ : Iris.Language.state Λ)
+    (l : Nat) (v : Iris.Language.val Λ) (hFresh : HeapLookup σ l = none) :
+    iProp.entails (Iris.state_interp Λ σ)
+      (bupd (iProp.sep (Iris.state_interp Λ (HeapInsert σ l v)) (pointsto l v)))
 
-axiom gen_heap_valid {Λ : Type} [Language Λ] (σ : Language.state Λ)
-    (l : Nat) (v : Language.val Λ) :
-    iProp.entails (iProp.sep (state_interp Λ σ) (pointsto l v))
+axiom gen_heap_valid {Λ : Type} [Iris.Language Λ] (σ : Iris.Language.state Λ)
+    (l : Nat) (v : Iris.Language.val Λ) :
+    iProp.entails (iProp.sep (Iris.state_interp Λ σ) (pointsto l v))
       (iProp.pure (HeapLookup σ l = some v))
 
-axiom gen_heap_update {Λ : Type} [Language Λ] (σ : Language.state Λ)
-    (l : Nat) (v v' : Language.val Λ) :
-    iProp.entails (iProp.sep (state_interp Λ σ) (pointsto l v))
-      (bupd (iProp.sep (state_interp Λ (HeapInsert σ l v')) (pointsto l v')))
+axiom gen_heap_update {Λ : Type} [Iris.Language Λ] (σ : Iris.Language.state Λ)
+    (l : Nat) (v v' : Iris.Language.val Λ) :
+    iProp.entails (iProp.sep (Iris.state_interp Λ σ) (pointsto l v))
+      (bupd (iProp.sep (Iris.state_interp Λ (HeapInsert σ l v')) (pointsto l v')))
